Ctl/Definition.v
@@ -1,18 +1,24 @@
 Require Import Ctl.Paths.
 Require Import BinaryRelations.
-Require Import Isomorphisms.
 
 Class transition {A} (R: relation A) := 
   {trans_serial: serial_witness R}.
 
-(* Definition tprop state := relation state -> state -> Prop. *)
+(* Note: none of the CTL formulas explicitly use the transition instance, but they do 
+   make recursive entailment assertions which implicitly pass the transition instance
+   forward.
 
+   Ultimately, the transition instance is only used by the theorems in Properties.v.
+   It is nonetheless important that a transition instance be mandated for entailments. 
+   Otherwise, the path-quantifying formulas would lose their current meaning.
+ *)
 Definition tprop state :=
   forall R: relation state,
     transition R ->
     state ->
     Prop.
 
+Declare Scope tprop_scope.
 Delimit Scope tprop_scope with tprop.
 Open Scope tprop_scope.
 
@@ -63,25 +69,25 @@ Notation "⟨ P ⟩"   := (tlift P)     (format "⟨ P ⟩"): tprop_scope.
 (* path-quantifying props *)
 
 Definition AX {state} (P: tprop state) : tprop state :=
-  fun R t s => forall s', R s s' -> R @s' ⊨ P.
+  fun R _ s => forall s', R s s' -> R @s' ⊨ P.
   
 Definition EX {state} (P: tprop state) : tprop state :=
-  fun R t s => exists s', R s s' /\ R @s' ⊨ P.
+  fun R _ s => exists s', R s s' /\ R @s' ⊨ P.
 
 Definition AG {state} (P: tprop state) : tprop state :=
-  fun R t s => forall (p: path R s) s', in_path s' p -> R @s' ⊨ P.
+  fun R _ s => forall (p: path R s) s', in_path s' p -> R @s' ⊨ P.
 
 Definition EG {state} (P: tprop state) : tprop state :=
-  fun R t s => exists p: path R s, forall s', in_path s' p -> R @s' ⊨ P.
+  fun R _ s => exists p: path R s, forall s', in_path s' p -> R @s' ⊨ P.
 
 Definition AF {state} (P: tprop state) : tprop state :=
-  fun R t s => forall p: path R s, exists s', in_path s' p /\ R @s' ⊨ P.
+  fun R _ s => forall p: path R s, exists s', in_path s' p /\ R @s' ⊨ P.
   
 Definition EF {state} (P: tprop state) : tprop state :=
-  fun R t s => exists (p: path R s) s', in_path s' p /\ R @s' ⊨ P.
+  fun R _ s => exists (p: path R s) s', in_path s' p /\ R @s' ⊨ P.
 
 Definition AU {state} (P Q: tprop state) : tprop state :=
-  fun R t s => forall p: path R s, exists sQ i,
+  fun R _ s => forall p: path R s, exists sQ i,
     in_path_at sQ i p /\ 
     (forall sP, in_path_before sP i p -> R @sP ⊨ P) /\ 
     R @sQ ⊨ Q.
@@ -97,7 +103,7 @@ Notation "A[ P 'U' Q ]" := (AU P Q) (at level 40, format "A[ P  'U'  Q ]") : tpr
 Notation "E[ P 'U' Q ]" := (EU P Q) (at level 40, format "E[ P  'U'  Q ]") : tprop_scope.
 
 Definition AW {state} (P Q: tprop state) : tprop state :=
-  fun R t s => R @s ⊨ A[P U Q] ∨ ¬AF P.
+  fun R _ s => R @s ⊨ A[P U Q] ∨ ¬AF P.
   (* fun R s => forall s' (seq: R#* s s'),
     (forall x, in_seq x seq -> R @x ⊨ P ∧ ¬Q) ->
     forall s'', 
