TransitionSystems.v
@@ -1,16 +1,14 @@
 Require Import BinaryRelations.
 
-(* Record state A B := mkState {global : A; local : B}.
-Definition transition A B := relation (state A B). *)
-
-Definition transition A B := relation (A * B).
+(* A transition relation over a global and local state *)
+Definition state_trans A B := relation (A * B).
 
 (* This mirrors Chlipala's definition of concurrent transitions in FRAP *)
-(* Can nested transitions have "globals" for various levels? *)
-Inductive either_transition {G A B} (R: transition G A) (Q: transition G B) : transition G (A * B) :=
+Inductive either_trans {G A B} (R: state_trans G A) (Q: state_trans G B)
+  : state_trans G (A * B) :=
   | step_l : forall g g' a a' b,
-      R (g,a) (g',a') -> either_transition R Q (g,(a,b)) (g',(a',b))
+      R (g,a) (g',a') -> either_trans R Q (g,(a,b)) (g',(a',b))
   | step_r : forall g g' a b b',
-      Q (g,b) (g',b') -> either_transition R Q (g,(a,b)) (g',(a,b')).
+      Q (g,b) (g',b') -> either_trans R Q (g,(a,b)) (g',(a,b')).
     
-Notation "R ⊔ S" := (either_transition R S) (at level 70).
+Notation "R ⊔ S" := (either_trans R S) (at level 70).
